\documentclass[UTF8]{ctexart}
\title{初等函数求导公式\&法则}
\author{AwtyvR}
\usepackage{amsmath}
\begin{document}
\maketitle

\Large

公式：

(1)$\frac{dC}{dx}=0$

(2)$\frac{d(x^a)}{dx}=ax^{a-1}(a\neq0\&x>0)$

(3)$\frac{d(ln(x))}{dx}=\frac{1}{x}(x>0)$

(4)$\frac{d(log_a(x))}{dx}=\frac{1}{x\space{}ln(a)}(a>0,a\neq1\&x>0)$

(5)$\frac{d(e^x)}{dx}=e^x$

(6)$\frac{d(a^x)}{dx}=a^xln(a)(a>0\&a\neq1)$

(7)$\frac{d(sin(x))}{dx}=cos(x)$

(8)$\frac{d(cos(x))}{dx}=-sin(x)$

(9)$\frac{d(tan(x))}{dx}=\frac{1}{cos^2(x)}$

(10)$\frac{d(cot(x))}{dx}=-\frac{1}{sin^2(x)}$

(11)$\frac{d(arcsin(x))}{dx}=\frac{1}{\sqrt{1-x^2}}(\lvert{x}\rvert<1)$

(12)$\frac{d(arccos(x))}{dx}=-\frac{1}{\sqrt{1-x^2}}(\lvert{x}\rvert<1)$

(13)$\frac{d(arctan(x))}{dx}=\frac{1}{x^2+1}$

(14)$\frac{d(arccot(x))}{dx}=-\frac{1}{x^2+1}$

法则：（注：以下用$f'(x)$代替$\frac{df}{dx}(x)$，用$()'$代替$\frac{d}{dx}$）

a.$({\alpha}f(x)+{\beta}g(x))'={\alpha}f'(x)+{\beta}g'(x)$

b.$(f(x)g(x))'=f'(x)g(x)+g'(x)f(x)$

c.$\bigl(\frac{f(x)}{g(x)}\bigr)'=\frac{f'(x)g(x)-g'(x)f(x)}{g^2(x)}$

d.$(f(g(x)))'=f'(g(x))g'(x)$

e.$(f^{-1}(x))'=\frac{1}{f'(f^{-1}(x))}$,其中$f(f^{-1}(x))=x$
\end{document}